src/json_theorems.v
@@ -3,53 +3,204 @@ Require Import json.
 From Coq Require Import Strings.String.
 From Coq Require Import ZArith.
 From Coq Require Import Lia.
-
-
-Lemma div_10_le : forall n time,
-  n <= S time -> n / 10 <= time.
-Proof.
-  intros [|n] time H. simpl. lia.
-  assert (S n / 10 < S n); try lia.
-  apply Nat.div_lt; lia.
-Qed.
-
-Lemma digit_iso : forall n, nat_of_ascii (ascii_of_nat (mod_10 n)) = Some (proj1_sig (mod_10 n)).
-Proof.
-  intros.
-  destruct (mod_10 n).
-  repeat match goal with
-         | m: nat  |- _  => destruct m; [ reflexivity | try lia ]
-         end.
-Defined.
-
-Lemma mod_10_correct : forall n, (proj1_sig (mod_10 n)) = n mod 10.
-Proof.
-  intros. unfold mod_10. reflexivity.
-Defined.
-  
-Theorem parse_nat_aux_iso : forall time n acc,
-    (n <= time) -> 
-    nat_of_string_aux 0 (string_of_nat_aux time n acc) = nat_of_string_aux n acc.
-Proof.
-  intros time.
-  induction time as [|time' Htime]; intros n acc H.
-  - simpl. inversion H. reflexivity.
-  - apply div_10_le in H. unfold string_of_nat_aux. destruct (n / 10) as [|n'] eqn: En'.
-    * unfold nat_of_string_aux. rewrite digit_iso. f_equal. pose (Nat.Div0.div_mod n 10) as N. rewrite En' in N. rewrite mod_10_correct. symmetry. apply N.
-    * rewrite Htime.
-      ** unfold nat_of_string_aux. rewrite digit_iso. f_equal. pose (Nat.Div0.div_mod n 10) as N. rewrite En' in N. rewrite mod_10_correct. symmetry. apply N.
-      ** apply H.
-Defined.
-
-Theorem parse_nat_isomorphic : forall (n: nat), parse_nat (string_of_nat n) = Ok(n, EmptyString).
-Proof.
-  intros.
-  unfold parse_nat. unfold string_of_nat.
-  apply parse_nat_aux_iso. reflexivity.
-Defined.
+From Coq Require Import Lists.List. Import ListNotations.
 
 Open Scope string_scope.
 
+Lemma parser_map_correct: forall T R I E (f: T -> R) s (p: @parser T I E),
+    (parser_map f p) s = fmap (fun '(v, rest) => (f v, rest)) (p s).
+Proof.
+  intros.
+  unfold parser_map, fmap.
+  destruct (p s) as [[val rest] |  err]; reflexivity.
+Defined.
+
+Lemma predicate_correct: forall T I E (p: @parser T I E) (pred: I -> bool) (err_handler: option I -> list E) v s rest,
+    Ok (v, rest) = predicate pred err_handler s ->
+    pred v = true.
+Proof.
+  intros.
+  unfold predicate in H.
+  
+  destruct s.
+  - discriminate H.
+  - destruct (pred i) eqn:Eq.
+    + inversion H. apply Eq.
+    + discriminate H.
+Defined.
+
+Lemma utf8_encode_correct : forall l (c: codepoint),
+    l = utf8_encode_codepoint c  ->
+    (exists b1 b2 b3 b4 b5 b6 b7,
+        l = [ Byte.of_bits (b7, (b6, (b5, (b4, (b3, (b2, (b1, false))))))) ]
+        /\ c = (false, b4_zero, b4_zero, b4_zero, (false, b1, b2, b3), (b4, b5, b6, b7)) )
+    \/ (exists b1 b2 b3 b4 b5 b6 b7 b8 b9 b10 b11,
+           l = [ Byte.of_bits (b5,  (b4,  (b3, (b2, (b1, (false,  (true, true)))))));
+                 Byte.of_bits (b11, (b10, (b9, (b8, (b7, (b6, (false, true))))))) ]
+           /\ c = (false, b4_zero, b4_zero, (false, b1, b2, b3), (b4, b5, b6, b7), (b8, b9, b10, b11))
+           /\ (b1 = true \/ b2 = true \/ b3 = true \/ b4 = true))
+    \/ (exists b1 b2 b3 b4 b5 b6 b7 b8 b9 b10 b11 b12 b13 b14 b15 b16,
+           l = [ Byte.of_bits (b4,  (b3,  (b2,  (b1,  (false,   (true, (true, true)))))));
+                 Byte.of_bits (b10, (b9,  (b8,  (b7,  (b6,  (b5,  (false, true)))))));
+                 Byte.of_bits (b16, (b15, (b14, (b13, (b12, (b11, (false, true)))))))]
+           /\ c = (false, b4_zero, (b1, b2, b3, b4), (b5, b6, b7, b8), (b9, b10, b11, b12), (b13, b14, b15, b16))
+           /\ (b1 = true \/ b2 = true \/ b3 = true \/ b4 = true \/ b5 = true))
+    \/ (exists b1 b2 b3 b4 b5 b6 b7 b8 b9 b10 b11 b12 b13 b14 b15 b16 b17 b18 b19 b20 b21,
+           l = [ Byte.of_bits (b3,  (b2,  (b1,  (false,   (true,  (true,   (true, true)))))));
+                 Byte.of_bits (b9,  (b8,  (b7,  (b6,  (b5,  (b4,  (false, true)))))));
+                 Byte.of_bits (b15, (b14, (b13, (b12, (b11, (b10, (false, true)))))));
+                 Byte.of_bits (b21, (b20, (b19, (b18, (b17, (b16, (false, true))))))) ]
+           /\ c = (b1, (b2, b3, b4, b5), (b6, b7, b8, b9), (b10, b11, b12, b13), (b14, b15, b16, b17), (b18, b19, b20, b21))
+           /\ (b1 = true \/ b2 = true \/ b3 = true \/ b4 = true \/ b5 = true)).
+Proof.
+  intros.
+  destruct c as [[[[[b21 [[[b20 b19] b18] b17]]
+                      [[[b16 b15] b14] b13]]
+                     [[[b12 b11] b10] b9]]
+                    [[[b8 b7] b6] b5]]
+                   [[[b4 b3] b2] b1]].
+  unfold utf8_encode_codepoint in H.
+  repeat match goal with
+         | [_: l = if ?bit then [ _; _; _; _ ] else ?rest |- _] => destruct bit; [ right; right; right; repeat eexists; [ apply H | auto ] | ]
+         | [_: l = if ?bit then [ _; _; _ ] else ?rest |- _] => destruct bit; [ right; right; left; repeat eexists; [ apply H | auto ] |  ]
+         | [_: l = if ?bit then [ _; _ ] else ?rest |- _] => destruct bit; [ right; left; repeat eexists; [ apply H | auto ] | ]
+         end.
+  left. repeat eexists. apply H.
+Defined.
+
+Theorem encoding_size_correct :
+  (forall b1 b2 b3 b4 b5 b6 b7,
+      encoding_size_from_header
+        (Byte.of_bits (b1, (b2, (b3, (b4, (b5, (b6, (b7, false)))))))) = Some (OneByte (b7, b6, b5, b4, b3, b2, b1)))
+  /\ (forall b1 b2 b3 b4 b5,
+         encoding_size_from_header
+           (Byte.of_bits (b1, (b2, (b3, (b4, (b5, (false, (true, true)))))))) = Some (TwoBytes (b5, b4, b3, b2, b1)))
+  /\ (forall b1 b2 b3 b4,
+         encoding_size_from_header
+           (Byte.of_bits (b1, (b2, (b3, (b4, (false, (true, (true, true)))))))) = Some (ThreeBytes (b4, b3, b2, b1)))
+  /\ (forall b1 b2 b3,
+         encoding_size_from_header
+        (Byte.of_bits (b1, (b2, (b3, (false, (true, (true, (true, true)))))))) = Some (FourBytes (b3, b2, b1))).
+Proof.
+  unfold encoding_size_from_header.
+  repeat split; intros; rewrite Byte.to_bits_of_bits.
+  - destruct b4; destruct b5; destruct b6; destruct b7; reflexivity.
+  - destruct b4; destruct b5; reflexivity.
+  - destruct b4; reflexivity.
+  - reflexivity.
+Defined.
+
+Theorem parse_continuation_correct: forall rest b1 b2 b3 b4 b5 b6,
+    parse_continuation (Byte.of_bits (b1, (b2, (b3, (b4, (b5, (b6, (false, true))))))) :: rest) = Ok ((b6, b5, b4, b3, b2, b1), rest).
+Proof.
+  intros.
+  unfold parse_continuation.
+  rewrite parser_map_correct.
+  unfold predicate. rewrite Byte.to_bits_of_bits.
+  unfold fmap.
+  unfold bind.
+  assert ((if true && negb false
+     then Ok (Byte.of_bits (b1, (b2, (b3, (b4, (b5, (b6, (false, true))))))), rest)
+     else
+      Err
+        [InvalidContinuationHeader
+           (Byte.of_bits (b1, (b2, (b3, (b4, (b5, (b6, (false, true))))))))]) = Ok (Byte.of_bits (b1, (b2, (b3, (b4, (b5, (b6, (false, true))))))), rest)) as G; try reflexivity.
+  rewrite G.
+  rewrite Byte.to_bits_of_bits.
+  reflexivity.
+Defined.
+  
+Theorem parse_codepoint_encode_correct : forall c rest, parse_codepoint ((utf8_encode_codepoint c) ++ rest)%list = Ok (c, rest).
+Proof.
+
+  Ltac no_overlongs :=
+    match goal with
+    | [ G: ?bit = true |- context[if ?bit then _ else _] ] => rewrite G; reflexivity
+    | |- context[if ?bit then _ else _] => destruct bit; [ reflexivity | no_overlongs ]
+    end.
+  intros.
+  destruct encoding_size_correct as [enc_one [enc_two [enc_three enc_four]]].
+  destruct (utf8_encode_correct (utf8_encode_codepoint c) c) as [? | [ ? | [ ? | [ ? ?]]]]; auto.
+  - destruct H as [b1 [b2 [b3 [b4 [b5 [b6 [b7 [eq c_eq]]]]]]]].
+    rewrite eq.
+    unfold parse_codepoint, parse_header.
+    unfold bind.
+    unfold app.
+    rewrite enc_one. simpl.
+    rewrite c_eq.
+    reflexivity.
+  - destruct H as [b1 [b2 [b3 [b4 [b5 [b6 [b7 [b8 [b9 [b10 [b11 [eq [c_eq no_overlong]]]]]]]]]]]]].
+    rewrite eq.
+    unfold parse_codepoint, parse_header.
+    unfold app.
+    rewrite enc_two.
+    rewrite c_eq.
+    unfold bind.
+    repeat rewrite parse_continuation_correct.
+    unfold codepoint_range_to_codepoint.
+    destruct no_overlong as [H | [H | [H | H]]]; no_overlongs.
+  - destruct H as [b1 [b2 [b3 [b4 [b5 [b6 [b7 [b8 [b9 [b10 [b11 [ b12 [b13 [b14 [b15 [b16 [eq [c_eq no_overlong]]]]]]]]]]]]]]]]]].
+    rewrite eq.
+    unfold parse_codepoint, parse_header.
+    unfold app.
+    rewrite enc_three.
+    rewrite c_eq.
+    unfold bind.
+    repeat rewrite parse_continuation_correct.
+    unfold codepoint_range_to_codepoint.
+    destruct no_overlong as [H | [H | [H | [H | H]]]]; no_overlongs.
+  - destruct H as [b2 [b3 [b4 [b5 [b6 [b7 [b8 [b9 [b10 [b11 [ b12 [b13 [b14 [b15 [b16 [b17 [b18 [b19 [b20 [b21 [eq [c_eq no_overlong]]]]]]]]]]]]]]]]]]]]]].
+    rewrite eq.
+    unfold parse_codepoint, parse_header.
+    unfold app.
+    rewrite enc_four.
+    rewrite c_eq.
+    unfold bind.
+    repeat rewrite parse_continuation_correct.
+    unfold codepoint_range_to_codepoint.
+    destruct no_overlong as [H | [H | [H | [H | H]]]]; no_overlongs.
+Defined.
+
+Lemma parse_single_codepoint_correct : forall c, parse_codepoint (utf8_encode_codepoint c) = Ok (c, []).
+Proof.
+  intros.
+  rewrite <- (List.app_nil_r (utf8_encode_codepoint c)).
+  apply (parse_codepoint_encode_correct c []).
+Defined.
+  
+Lemma many_codepoint_distributes : forall (c: codepoint) (cs: list codepoint),
+    many parse_codepoint (utf8_encode_codepoint c ++ concat (map utf8_encode_codepoint cs))%list =
+      let* (x, rest) := parse_codepoint (utf8_encode_codepoint c) in
+      let* (xs, rest) := many parse_codepoint (concat (map utf8_encode_codepoint cs)) in
+      Ok (x :: xs, rest).
+Proof.
+  induction cs.
+  - simpl.
+    rewrite app_nil_r.
+    rewrite parse_single_codepoint_correct. unfold bind.
+    destruct (utf8_encode_correct (utf8_encode_codepoint c) c) as [? | [ ? | [ ? | [ ? ?]]]]; auto;
+      [ destruct H as [b1 [b2 [b3 [b4 [b5 [b6 [b7 [eq c_eq]]]]]]]]
+      | destruct H as [b1 [b2 [b3 [b4 [b5 [b6 [b7 [b8 [b9 [b10 [b11 [eq [c_eq no_overlong]]]]]]]]]]]]]
+      | destruct H as [b1 [b2 [b3 [b4 [b5 [b6 [b7 [b8 [b9 [b10 [b11 [ b12 [b13 [b14 [b15 [b16 [eq [c_eq no_overlong]]]]]]]]]]]]]]]]]]
+      | destruct H as [b2 [b3 [b4 [b5 [b6 [b7 [b8 [b9 [b10 [b11 [ b12 [b13 [b14 [b15 [b16 [b17 [b18 [b19 [b20 [b21 [eq [c_eq no_overlong]]]]]]]]]]]]]]]]]]]]]]
+      ]; rewrite eq; rewrite c_eq. unfold many, many_aux. unfold bind.
+  
+  Admitted.
+
+ 
+Theorem encode_decode_correct : forall u, utf8_decode (utf8_encode u) = Ok (u, []).
+Proof.
+  intros.
+  unfold utf8_encode, utf8_decode.
+
+  induction u; auto. simpl.
+  rewrite many_codepoint_distributes.
+  rewrite parse_single_codepoint_correct.
+  rewrite IHu.
+  reflexivity.
+Qed.
+
+   
 Theorem parse_null_isomorphic : parse_null "null" = Ok((JNull, "")).
   reflexivity.
 Qed.
@@ -59,6 +210,8 @@ Qed.
 Theorem parse_false_isomorphic : parse_false "false" = Ok((JFalse, "")).
   reflexivity.
 Qed.
+
+
 
 Theorem parser_map_correct { A B }: forall (f: A -> B) (p: @parser A) (s: string),
     parser_map f p s = fmap (fun '(x, rest) => (f x, rest)) (p s).
